SV_float.v
@@ -1,5 +1,5 @@
 Set Implicit Arguments.
-From SLF Require Import LabType Fun LibSepFmap Sum Unary.
+From SLF Require Import LabType Fun LibSepFmap Sum Unary Dotprod_float Prelude.
 From SLF Require Import LibWP LibSepSimpl LibSepReference LibSepTLCbuffer Struct Struct2 Loops Loops2 ListCommon.
 From mathcomp Require Import ssreflect ssrfun zify.
 Hint Rewrite conseq_cons' : rew_listx.
@@ -8,67 +8,7 @@ From Coq Require Import Permutation.
 
 Open Scope Z_scope.
 
-(* TODO maybe move this somewhere else *)
-Module incr_float.
-
-Section incr_float. 
-
-Context {D : Type}.
-
-Definition func :=
-  (<{ fun "real_j" "x" =>
-      let "tmp1" = ! "real_j" in
-      let "tmp2" = "tmp1" .+ "x" in
-      "real_j" := "tmp2" }>).
-
-Lemma spec `{Inhab D} (pj0 : loc) (d : D) (j x : binary64) :
-  htriple (single d tt)
-  (fun=> func pj0 x) 
-  (pj0 ~(d)~> val_float j)
-    (fun=> pj0 ~(d)~> val_float (j + x)%F64).
-Proof. by do 3 (xwp; xapp). Qed.
-
-End incr_float.
-End incr_float.
-
-Notation "k '.+=' x" :=
-  (incr_float.func k x)
-  (in custom trm at level 58, format "k  .+=  x") : trm_scope.
-
-Module fma.
-
-Section fma. 
-
-Context {D : Type}.
-
-Definition func :=
-  (<{ fun "z" "x" "y" =>
-      let "tmp1" = "x" .* "y" in
-      let "tmp2" = ! "z" in
-      let "tmp2" = val_float_fma "tmp1" "tmp2" in
-      "z" := "tmp2" }>).
-
-Lemma spec `{Inhab D} (pj0 : loc) (d : D) (x y z : binary64) :
-  htriple (single d tt)
-  (fun=> func pj0 x y) 
-  (pj0 ~(d)~> val_float z)
-    (fun=> pj0 ~(d)~> val_float (@BFMA _ Tdouble x y z)).
-Proof. by do 4 (xwp; xapp). Qed.
-
-End fma.
-End fma.
-
 Coercion to_float : val >-> binary64.
-
-Lemma to_float_if P a b : 
-  to_float (If P then a else b) = If P then a else b.
-Proof. by case: classicT. Qed.
-
-Fact fold_left_map {A B C : Type} (l : list B) (g : B -> C) (f : A -> C -> A) (s : A) :
-  List.fold_left (fun a b => f a (g b)) l s = List.fold_left f (List.map g l) s.
-Proof.
-  revert s. induction l as [ | x l IH ] using List.rev_ind; intros; rewrite ?List.map_app ?List.fold_left_app /= ?IH; auto. 
-Qed. 
 
 (*
 (* This is not doable ... *)
@@ -85,116 +25,6 @@ Proof.
 Admitted.
 *)
 
-Definition Sum_fma {A : Type} (s : binary64) (l : list A) (f : A -> binary64 * binary64) : binary64 := 
-  List.fold_left (fun acc a => (@BFMA _ Tdouble (f a).1 (f a).2 acc)%F64) l s.
-
-Lemma Sum_fma_filter0_feq {A : Type} (p : A -> bool) : forall (s : binary64) (l : list A) (f : A -> binary64 * binary64), 
-  (forall a, List.In a l -> p a = false -> (f a).1 = float_unit \/ (f a).2 = float_unit) -> 
-  (forall a, List.In a l -> @finite Tdouble (f a).1 /\ @finite Tdouble (f a).2) ->
-  @feq Tdouble (Sum_fma s l f) (Sum_fma s (List.filter p l) f).
-Proof.
-  move=> s l. move: s.
-  induction l as [ | a l IH ] using List.rev_ind; intros; auto.
-  unfold Sum_fma in *. rewrite List.fold_left_app List.filter_app /=. 
-  destruct (p a) eqn:Ef; rewrite ?IH //= ?List.fold_left_app //=.
-  all: try (move=> a0 Hin; (apply H + apply H0); rewrite List.in_app_iff; tauto).
-  specialize (H0 a). rewrite List.in_app_iff /= /finite in H0. 
-  specialize (H0 (or_intror (or_introl eq_refl))). 
-  apply H in Ef. 2: rewrite List.in_app_iff /=; tauto.
-  destruct H0, Ef as [ -> | -> ]; rewrite ?BFMA_zero1 ?BFMA_zero2 //=.
-Qed.
-
-Lemma pair_fst_If {A B : Type} P (a b : A) (c : B) : 
-  (If P then a else b, c) = If P then (a, c) else (b, c).
-Proof. by case_if. Qed.
-
-Lemma Sum_fma_eq {A : Type} (s : binary64) (l : list A) (f g : A -> binary64 * binary64) :
-  (forall a, List.In a l -> f a = g a) -> Sum_fma s l f = Sum_fma s l g.
-Proof.
-  intros H. revert s. induction l; intros; simpl; auto. rewrite ?H ?IHl; simpl; auto.
-  move=>*. rewrite H /=; tauto.
-Qed.
-
-Lemma Sum_fma_feq_base {A : Type} (s s' : binary64) (l : list A) (f : A -> binary64 * binary64) :
-  @feq Tdouble s s' -> @feq Tdouble (Sum_fma s l f) (Sum_fma s' l f).
-Proof. revert s s'. induction l; intros; simpl; auto. by apply IHl, BFMA_mor. Qed.
-
-Lemma Sum_fma_feq {A : Type} (s : binary64) (l : list A) (f g : A -> binary64 * binary64) :
-  (forall a, List.In a l -> @feq Tdouble (f a).1 (g a).1 /\ @feq Tdouble (f a).2 (g a).2) -> 
-  @feq Tdouble (Sum_fma s l f) (Sum_fma s l g).
-Proof.
-  intros H. revert s. induction l; intros; simpl; auto. 
-  pose proof (H a (or_introl eq_refl)) as (H1 & H2).
-  etransitivity. 1: apply Sum_fma_feq_base, BFMA_mor; eauto.
-  apply IHl=> a' Hin. apply H; simpl; auto.
-Qed.
-
-Corollary Sum_fma_filter_If {A : Type} (P : A -> Prop) (s : binary64) (l : list A) (f g : A -> binary64) 
-  (Hfinf : forall a, List.In a l -> P a -> @finite Tdouble (f a))
-  (Hfing : forall a, List.In a l -> @finite Tdouble (g a)) :
-  @feq Tdouble (Sum_fma s l (fun i => If P i then (f i, g i) else (float_unit, g i))) 
-    (Sum_fma s (List.filter (fun i => isTrue (P i)) l) (fun i => (f i, g i))).
-Proof.
-  rewrite -> Sum_fma_filter0_feq with (p:=fun i => isTrue (P i)).
-  2:{ intros. rewrite -> isTrue_eq_false_eq in *. case_if; auto. }
-  2:{ intros. case_if; simpl; auto. }
-  rewrite -> Sum_fma_eq with (g:=fun i => (f i, g i)). 
-  2:{ intros ? Hin%List.filter_In. rewrite isTrue_eq_true_eq in Hin. case_if; eqsolve. }
-  reflexivity.
-Qed.
-
-Corollary Sum_fma_filter_If' {A : Type} (P : A -> Prop) (s : binary64) (l : list A) (f : A -> val) g
-  (Hfinf : forall a, List.In a l -> P a -> @finite Tdouble (to_float (f a)))
-  (Hfing : forall a, List.In a l -> @finite Tdouble ( (g a))) :
-  @feq Tdouble (Sum_fma s l (fun i => (to_float (If P i then f i else float_unit), (g i)))) 
-    (Sum_fma s (List.filter (fun i => isTrue (P i)) l) (fun i => (to_float (f i), g i))).
-Proof.
-  erewrite Sum_fma_eq; [ | move=> i0 ?; rewrite to_float_if pair_fst_If; reflexivity ].
-  rewrite Sum_fma_filter_If -?sorted_bounded_sublist //.
-Qed.
-
-Lemma Sum_fma_list_interval (s : binary64) (l : list int) (f : int -> binary64 * binary64) 
-  lb rb (H1 : 0 <= lb) (H2 : lb <= rb) (H3 : rb <= List.length l) :
-  Sum_fma s (list_interval (abs lb) (abs rb) l) f = Sum_fma s (lof id (rb - lb)) (fun i => f (l[i + lb])).
-Proof.
-  unfold Sum_fma.
-  match goal with 
-    |- List.fold_left ?ff _ _ = _ => 
-      pose proof (fold_left_map (lof id (rb - lb)) (fun a : int => l[a + lb]) ff s) as Htmp
-  end.
-  simpl in Htmp. rewrite Htmp. f_equal.
-  assert (List.length (lof id (rb - lb)) = rb - lb :> int) as Hl1 by (rewrite length_lof; math).
-  assert (List.length (list_interval (abs lb) (abs rb) l) = rb - lb :> int) as Hl2 by (rewrite list_interval_length; math).
-  apply (List.nth_ext _ _ 0 0). 
-  1: rewrite List.map_length; math.
-  intros n Hlt. replace n with (abs n)%nat by math.
-  rewrite (nth_map_lt 0) -?list_interval_nth ?nth_lof; try math. f_equal. math.
-Qed.
-
-Lemma Sum_fma_lof {A} (f : int -> A) s n (g : A -> _) : 
-  Sum_fma s (projT1 (list_of_fun' f n)) g = 
-  Sum_fma s (lof id n) (fun x => g (f x)).
-Proof.
-  unfold Sum_fma.
-  match goal with 
-    |- List.fold_left ?ff _ _ = _ => pose proof (fold_left_map (lof id n) f ff s) as Htmp
-  end.
-  simpl in Htmp. rewrite Htmp. f_equal. apply lof_indices'.
-Qed.
-
-(*
-Lemma Sum_fma_filter_If {A : Type} (P : int -> Prop) (f g : A -> binary64 * binary64) : 
-  forall (s : binary64) (l : list A) (f : A -> binary64 * binary64), 
-  (forall a, List.In a l -> p a = false -> (f a).1 = float_unit \/ (f a).2 = float_unit) -> 
-  (forall a, List.In a l -> @finite Tdouble (f a).1 /\ @finite Tdouble (f a).2) ->
-  @feq Tdouble (Sum_fma s l f) (Sum_fma s (List.filter p l) f).
-Proof.
-*)
-
-Fact finite_suffcond (l : list binary64) n (H : forall x, List.In x l -> @finite Tdouble x) :
-  @finite Tdouble (List.nth n l float_unit).
-Proof. destruct (List.nth_in_or_default n l float_unit) as [ | -> ]; auto. by compute. Qed.
-
 Module sv_float.
 
 Notation "H1 '\\*' H2" := (hstar H1 H2)
@@ -209,7 +39,7 @@ Notation "'dvec'" := ("d_vec":var) (in custom trm at level 0) : trm_scope.
 Notation "'xlb'" := ("l_b":var) (in custom trm at level 0) : trm_scope.
 Notation "'xrb'" := ("r_b":var) (in custom trm at level 0) : trm_scope.
 
-Import List Vars.
+Import List Vars list_interval_notation.
 
 Context (xind : list int).
 Context (xval : list binary64).
@@ -219,10 +49,10 @@ Hypothesis (len : rb - lb = N).
 Hypotheses (bounds_l: 0 <= lb) (bounds_r: lb <= rb).
 Hypothesis len_xind : rb <= length xind.
 Hypothesis len_xval : rb <= length xval.
-Hypothesis nodup_xind : NoDup (list_interval (abs lb) (abs rb) xind).
-Hypothesis sorted_xind : sorted (list_interval (abs lb) (abs rb) xind). (* TODO possibly remove nodup_xind since sorted_xind subsumes it? *)
-Hypothesis xind_leq : forall x, In x (list_interval (abs lb) (abs rb) xind) -> 0 <= x < M.
-Hypothesis xval_finite : forall x, In x (list_interval (abs lb) (abs rb) xval) -> @finite Tdouble x.
+Hypothesis nodup_xind : NoDup (xind [[ lb -- rb ]]).
+Hypothesis sorted_xind : sorted (xind [[ lb -- rb ]]). (* TODO possibly remove nodup_xind since sorted_xind subsumes it? *)
+Hypothesis xind_leq : forall x, In x (xind [[ lb -- rb ]]) -> 0 <= x < M.
+Hypothesis xval_finite : forall x, In x (xval [[ lb -- rb ]]) -> @finite Tdouble x.
 
 Tactic Notation "seclocal_solver" :=
   first [ rewrite list_interval_nth'; auto; math
@@ -257,12 +87,12 @@ Qed.
 
 Lemma get_spec_in {D : Type} `{Inhab D} (x_ind x_val : loc) i d : 
   @htriple D (single d tt) 
-    (fun=> get (List.nth (abs i) (list_interval (abs lb) (abs rb) xind) 0) x_ind x_val lb rb)
+    (fun=> get (List.nth (abs i) (xind [[ lb -- rb ]]) 0) x_ind x_val lb rb)
     (\[0 <= i < N] \*
       harray_int xind x_ind d \* 
       harray_float xval x_val d)
     (fun hr => 
-     \[hr = fun=> List.nth (abs i) (list_interval (abs lb) (abs rb) xval) float_unit] \* 
+     \[hr = fun=> List.nth (abs i) (xval [[ lb -- rb ]]) float_unit] \* 
       harray_int xind x_ind d \* 
       harray_float xval x_val d).
 Proof with seclocal_solver.
@@ -276,7 +106,7 @@ Qed.
 Lemma get_spec_out_unary {D : Type} `{Inhab D} (x_ind x_val : loc) (i : int) d : 
   @htriple D (single d tt) 
     (fun=> get i x_ind x_val lb rb)
-    (\[~ In i (list_interval (abs lb) (abs rb) xind)] \*
+    (\[~ In i (xind [[ lb -- rb ]])] \*
       harray_int xind x_ind d \* 
       harray_float xval x_val d)
     (fun hr => 
@@ -295,7 +125,7 @@ Local Notation D := (labeled int).
 Lemma get_spec_out `{Inhab D} fs (x_ind x_val : loc) : 
   @htriple D fs
     (fun i => get (eld i) x_ind x_val lb rb)
-    (\[forall d, indom fs d -> ~ In (eld d) (list_interval (abs lb) (abs rb) xind)] \*
+    (\[forall d, indom fs d -> ~ In (eld d) (xind [[ lb -- rb ]])] \*
       (\*_(d <- fs) harray_int xind x_ind d) \* 
        \*_(d <- fs) harray_float xval x_val d)
     (fun hr => 
@@ -329,9 +159,6 @@ Definition sum :=
   let n := constr:(S1) in
   xfocus n; tac; try(
   first [xunfocus | xcleanup n]; simpl; try apply xnwp0_lemma). *)
-Lemma val_float_eq i j : 
-  (val_float i = val_float j) = (i = j).
-Proof. by extens; split=> [[]|]->. Qed.
 
 Ltac fold' := 
   rewrite ?label_single ?wp_single ?val_float_eq
@@ -354,8 +181,6 @@ Proof.
   rewrite update_empty SumUpdate; [ rewrite Sum0 Z.add_0_l; reflexivity | auto ].
 Qed.
 *)
-
-Notation "l '[[' i '--' j ']]' " := (list_interval (abs i) (abs j) l) (at level 5).
 
 (*
 Lemma sum_spec `{Inhab D} (x_ind x_val : loc) : 
