Prelude.v
@@ -1,0 +1,7 @@
+Set Implicit Arguments.
+From SLF Require Import LibReflect.
+From mathcomp Require Import ssreflect ssrfun zify.
+
+Ltac bool_rew := 
+  rewrite ?false_eq_isTrue_eq ?istrue_isTrue_eq 
+    ?true_eq_isTrue_eq -?(isTrue_and, isTrue_not, isTrue_or) ?not_isTrueE.
